block_equiv_checker.v
@@ -1,0 +1,772 @@
+Require Import Bool.
+Require Import List.
+ 
+Require Import FORVES2.program.
+Import Program.
+
+Require Import FORVES2.stack_operation_instructions.
+Import StackOpInstrs.
+
+Require Import FORVES2.execution_state.
+Import ExecutionState.
+
+Require Import FORVES2.concrete_interpreter.
+Import ConcreteInterpreter.
+
+Require Import FORVES2.optimizations_def.
+Import Optimizations_Def.
+
+Require Import FORVES2.optimizations.add_zero.
+Import Opt_add_zero.
+Require Import FORVES2.optimizations.eval.
+Import Opt_eval.
+Require Import FORVES2.optimizations.not_not.
+Import Opt_not_not.
+Require Import FORVES2.optimizations.and_and.
+Import Opt_and_and.
+Require Import FORVES2.optimizations.and_origin.
+Import Opt_and_origin.
+Require Import FORVES2.optimizations.mul_shl.
+Import Opt_mul_shl.
+Require Import FORVES2.optimizations.div_shl.
+Import Opt_div_shl.
+Require Import FORVES2.optimizations.shr_zero_x.
+Import Opt_shr_zero_x.
+Require Import FORVES2.optimizations.shr_x_zero.
+Import Opt_shr_x_zero.
+Require Import FORVES2.optimizations.eq_zero.
+Import Opt_eq_zero.
+Require Import FORVES2.optimizations.sub_x_x.
+Import Opt_sub_x_x.
+Require Import FORVES2.optimizations.and_zero.
+Import Opt_and_zero.
+Require Import FORVES2.optimizations.div_one.
+Import Opt_div_one.
+Require Import FORVES2.optimizations.lt_x_one.
+Import Opt_lt_x_one.
+Require Import FORVES2.optimizations.gt_one_x.
+Import Opt_gt_one_x.
+Require Import FORVES2.optimizations.and_address.
+Import Opt_and_address.
+Require Import FORVES2.optimizations.mul_one.
+Import Opt_mul_one.
+Require Import FORVES2.optimizations.iszero_gt.
+Import Opt_iszero_gt.
+Require Import FORVES2.optimizations.eq_iszero.
+Import Opt_eq_iszero.
+Require Import FORVES2.optimizations.and_caller.
+Import Opt_and_caller.
+Require Import FORVES2.optimizations.iszero3.
+Import Opt_iszero3.
+Require Import FORVES2.optimizations.add_sub.
+Import Opt_add_sub.
+Require Import FORVES2.optimizations.shl_zero_x.
+Import Opt_shl_zero_x.
+Require Import FORVES2.optimizations.sub_zero.
+Import Opt_sub_zero.
+Require Import FORVES2.optimizations.shl_x_zero.
+Import Opt_shl_x_zero.
+Require Import FORVES2.optimizations.mul_zero.
+Import Opt_mul_zero.
+Require Import FORVES2.optimizations.div_x_x.
+Import Opt_div_x_x.
+Require Import FORVES2.optimizations.div_zero.
+Import Opt_div_zero.
+Require Import FORVES2.optimizations.mod_one.
+Import Opt_mod_one.
+Require Import FORVES2.optimizations.mod_zero.
+Import Opt_mod_zero.
+Require Import FORVES2.optimizations.mod_x_x.
+Import Opt_mod_x_x.
+Require Import FORVES2.optimizations.exp_x_zero.
+Import Opt_exp_x_zero.
+Require Import FORVES2.optimizations.exp_x_one.
+Import Opt_exp_x_one.
+Require Import FORVES2.optimizations.exp_one_x.
+Import Opt_exp_one_x.
+Require Import FORVES2.optimizations.exp_zero_x.
+Import Opt_exp_zero_x.
+Require Import FORVES2.optimizations.exp_two_x.
+Import Opt_exp_two_x.
+Require Import FORVES2.optimizations.gt_zero_x.
+Import Opt_gt_zero_x.
+Require Import FORVES2.optimizations.gt_x_x.
+Import Opt_gt_x_x.
+Require Import FORVES2.optimizations.lt_x_zero.
+Import Opt_lt_x_zero.
+Require Import FORVES2.optimizations.lt_x_x.
+Import Opt_lt_x_x.
+Require Import FORVES2.optimizations.eq_x_x.
+Import Opt_eq_x_x.
+Require Import FORVES2.optimizations.iszero_sub.
+Import Opt_iszero_sub.
+Require Import FORVES2.optimizations.iszero_lt.
+Import Opt_iszero_lt.
+Require Import FORVES2.optimizations.iszero_xor.
+Import Opt_iszero_xor.
+Require Import FORVES2.optimizations.iszero2_gt.
+Import Opt_iszero2_gt.
+Require Import FORVES2.optimizations.iszero2_lt.
+Import Opt_iszero2_lt.
+Require Import FORVES2.optimizations.iszero2_eq.
+Import Opt_iszero2_eq.
+Require Import FORVES2.optimizations.xor_x_x.
+Import Opt_xor_x_x.
+Require Import FORVES2.optimizations.xor_zero.
+Import Opt_xor_zero.
+Require Import FORVES2.optimizations.xor_xor.
+Import Opt_xor_xor.
+Require Import FORVES2.optimizations.or_or.
+Import Opt_or_or.
+Require Import FORVES2.optimizations.or_and.
+Import Opt_or_and.
+Require Import FORVES2.optimizations.and_or.
+Import Opt_and_or.
+Require Import FORVES2.optimizations.and_not.
+Import Opt_and_not.
+Require Import FORVES2.optimizations.or_not.
+Import Opt_or_not.
+Require Import FORVES2.optimizations.or_x_x.
+Import Opt_or_x_x.
+Require Import FORVES2.optimizations.and_x_x.
+Import Opt_and_x_x.
+Require Import FORVES2.optimizations.or_zero.
+Import Opt_or_zero.
+Require Import FORVES2.optimizations.or_ffff.
+Import Opt_or_ffff.
+Require Import FORVES2.optimizations.and_ffff.
+Import Opt_and_ffff.
+Require Import FORVES2.optimizations.and_coinbase.
+Import Opt_and_coinbase.
+Require Import FORVES2.optimizations.balance_address.
+Import Opt_balance_address.
+Require Import FORVES2.optimizations.slt_x_x.
+Import Opt_slt_x_x.
+Require Import FORVES2.optimizations.sgt_x_x.
+Import Opt_sgt_x_x.
+
+Require Import FORVES2.symbolic_execution.
+Import SymbolicExecution.
+
+Require Import FORVES2.storage_ops_solvers.
+Import StorageOpsSolvers.
+
+Require Import FORVES2.storage_ops_solvers_impl.
+Import StorageOpsSolversImpl.
+
+Require Import FORVES2.memory_ops_solvers.
+Import MemoryOpsSolvers.
+
+Require Import FORVES2.memory_ops_solvers_impl.
+Import MemoryOpsSolversImpl.
+
+Require Import FORVES2.symbolic_state_cmp.
+Import SymbolicStateCmp.
+
+Require Import FORVES2.valid_symbolic_state.
+Import ValidSymbolicState.
+
+Require Import FORVES2.symbolic_execution_soundness.
+Import SymbolicExecutionSoundness.
+
+Require Import FORVES2.symbolic_state_eval.
+Import SymbolicStateEval.
+
+Require Import FORVES2.symbolic_state.
+Import SymbolicState.
+
+Require Import FORVES2.symbolic_state_cmp_impl.
+Import SymbolicStateCmpImpl.
+
+Require Import FORVES2.sstack_val_cmp_impl.
+Import SStackValCmpImpl.
+
+Require Import FORVES2.sstack_val_cmp_impl_soundness.
+Import SStackValCmpImplSoundness.
+
+Require Import FORVES2.sha3_cmp_impl.
+Import SHA3CmpImpl.
+
+Require Import FORVES2.sha3_cmp_impl_soundness.
+Import SHA3CmpImplSoundness.
+
+Require Import FORVES2.storage_cmp_impl.
+Import StorageCmpImpl.
+
+Require Import FORVES2.storage_cmp_impl_soundness.
+Import StorageCmpImplSoundness.
+
+
+Require Import FORVES2.memory_cmp_impl.
+Import MemoryCmpImpl.
+
+Require Import FORVES2.memory_cmp_impl_soundness.
+Import MemoryCmpImplSoundness.
+
+Require Import FORVES2.storage_ops_solvers_impl.
+Import StorageOpsSolversImpl.
+
+Require Import FORVES2.storage_ops_solvers_impl_soundness.
+Import StorageOpsSolversImplSoundness.
+
+Require Import FORVES2.memory_ops_solvers_impl.
+Import MemoryOpsSolversImpl.
+
+Require Import FORVES2.memory_ops_solvers_impl_soundness.
+Import MemoryOpsSolversImplSoundness.
+
+Require Import FORVES2.symbolic_state_cmp_impl_soundness.
+Import SymbolicStateCmpImplSoundness.
+
+Require Import FORVES2.misc.
+Import Misc.
+
+Require Import FORVES2.constraints.
+Import Constraints.
+
+From Coq Require Import Lists.List. Import ListNotations.
+
+Module BlockEquivChecker.
+
+
+  (* mload solvers *)
+  Inductive mload_solver_v :=
+  | MLoadSolver (f: mload_solver_ext_type) (H_snd: mload_solver_ext_snd f).
+
+  Inductive available_mload_solvers :=
+  | MLoadSolver_Trivial
+  | MLoadSolver_Basic.
+
+  Definition get_mload_solver (tag: available_mload_solvers) : mload_solver_v :=
+    match tag with
+    | MLoadSolver_Trivial => MLoadSolver trivial_mload_solver trivial_mload_solver_snd
+    | MLoadSolverStrgUpdater_Basic => MLoadSolver basic_mload_solver basic_mload_solver_snd
+  end.
+
+  (* sload solvers *)
+  Inductive sload_solver_v :=
+  | SLoadSolver (f: sload_solver_ext_type) (H_snd: sload_solver_ext_snd f).
+
+  Inductive available_sload_solvers :=
+  | SLoadSolver_Trivial
+  | SLoadSolver_Basic.
+
+  Definition get_sload_solver (tag: available_sload_solvers) : sload_solver_v :=
+    match tag with
+    | SLoadSolver_Trivial => SLoadSolver trivial_sload_solver trivial_sload_solver_snd
+    | SLoadSolverStrgUpdater_Basic => SLoadSolver basic_sload_solver basic_sload_solver_snd
+  end.
+
+  (* memory updaters *)
+  Inductive smemory_updater_v :=
+  | SMemUpdater (f: smemory_updater_ext_type) (H_snd: smemory_updater_ext_snd f).
+
+  Inductive available_smemory_updaters :=
+  | SMemUpdater_Trivial
+  | SMemUpdater_Basic.
+
+  Definition get_smemory_updater (tag: available_smemory_updaters) : smemory_updater_v :=
+    match tag with
+    | SMemUpdater_Trivial => SMemUpdater trivial_smemory_updater trivial_smemory_updater_snd
+    | SMemUpdater_Basic => SMemUpdater basic_smemory_updater basic_smemory_updater_snd
+  end.
+
+  (* storage updaters *)
+  Inductive sstorage_updater_v :=
+  | SStrgUpdater (f: sstorage_updater_ext_type) (H_snd: sstorage_updater_ext_snd f).
+
+  Inductive available_sstorage_updaters :=
+  | SStrgUpdater_Trivial
+  | SStrgUpdater_Basic.
+
+  Definition get_sstorage_updater (tag: available_sstorage_updaters) : sstorage_updater_v :=
+    match tag with
+    | SStrgUpdater_Trivial => SStrgUpdater trivial_sstorage_updater trivial_sstorage_updater_snd
+    | SStrgUpdater_Basic => SStrgUpdater basic_sstorage_updater basic_sstorage_updater_snd
+  end.
+
+
+
+  
+  (* Memory comparators *)
+  Inductive smemory_cmp_v :=
+  | SMemCmp (f: smemory_cmp_ext_t) (H_snd: safe_smemory_cmp_ext_wrt_sstack_value_cmp f).
+
+  Inductive available_memory_cmp :=
+  | SMemCmp_Trivial
+  | SMemCmp_Basic
+  | SMemCmp_PO.
+
+  Definition get_memory_cmp (tag: available_memory_cmp) : smemory_cmp_v :=
+    match tag with
+    | SMemCmp_Trivial => SMemCmp trivial_memory_cmp trivial_memory_cmp_snd
+    | SMemCmp_Basic => SMemCmp basic_memory_cmp basic_memory_cmp_snd
+    | SMemCmp_PO => SMemCmp po_memory_cmp po_memory_cmp_snd
+  end.
+
+  (* Storage comparators *)
+  Inductive sstorage_cmp_v :=
+  | SStrgCmp (f: sstorage_cmp_ext_t) (H_snd: safe_sstorage_cmp_ext_wrt_sstack_value_cmp f).
+
+  Inductive available_storage_cmp :=
+  | SStrgCmp_Trivial
+  | SStrgCmp_Basic
+  | SStrgCmp_PO.
+  
+
+  Definition get_storage_cmp (tag: available_storage_cmp) : sstorage_cmp_v :=
+    match tag with
+    | SStrgCmp_Trivial => SStrgCmp trivial_storage_cmp trivial_storage_cmp_snd
+    | SStrgCmp_Basic => SStrgCmp basic_storage_cmp basic_storage_cmp_snd
+    | SStrgCmp_PO => SStrgCmp po_storage_cmp po_storage_cmp_snd
+  end.
+
+
+  (* SHA3 comparators *)
+  Inductive sha3_cmp_v :=
+  | SHA3Cmp (f: sha3_cmp_ext_t) (H_snd: safe_sha3_cmp_ext_wrt_sstack_value_cmp f).
+
+  Inductive available_sha3_cmp :=
+  | SHA3Cmp_Trivial.
+
+  Definition get_sha3_cmp (tag: available_sha3_cmp) : sha3_cmp_v :=
+    match tag with
+    | SHA3Cmp_Trivial => SHA3Cmp trivial_sha3_cmp trivial_sha3_cmp_snd
+  end.
+
+
+  (* sstack_val comparators *)
+  Inductive sstack_val_cmp_v :=
+  | SStackValCmp (f: sstack_val_cmp_ext_2_t) (H_snd: safe_sstack_value_cmp_wrt_others f) (H_d0_snd: sstack_val_cmp_fail_for_d_eq_0 f).
+
+  Inductive available_sstack_val_cmp :=
+  | SStackValCmp_Trivial
+  | SStackValCmp_Basic.
+
+  Definition get_sstack_val_cmp (tag: available_sstack_val_cmp) : sstack_val_cmp_v :=
+    match tag with
+    | SStackValCmp_Trivial => SStackValCmp trivial_compare_sstack_val trivial_compare_sstack_val_snd trivial_compare_sstack_val_d0_snd
+    | SStackValCmp_Basic => SStackValCmp basic_compare_sstack_val basic_compare_sstack_val_snd basic_compare_sstack_val_d0_snd
+  end.
+  
+  
+Inductive available_optimization_step :=
+| OPT_eval
+| OPT_add_zero
+| OPT_not_not
+| OPT_and_and
+| OPT_and_origin
+| OPT_mul_shl
+| OPT_div_shl
+| OPT_shr_zero_x
+| OPT_shr_x_zero
+| OPT_eq_zero
+| OPT_sub_x_x
+| OPT_and_zero
+| OPT_div_one
+| OPT_lt_x_one
+| OPT_gt_one_x
+| OPT_and_address
+| OPT_mul_one
+| OPT_iszero_gt
+| OPT_eq_iszero
+| OPT_and_caller
+| OPT_iszero3
+| OPT_add_sub
+| OPT_shl_zero_x
+| OPT_sub_zero
+| OPT_shl_x_zero
+| OPT_mul_zero
+| OPT_div_x_x
+| OPT_div_zero
+| OPT_mod_one
+| OPT_mod_zero
+| OPT_mod_x_x
+| OPT_exp_x_zero
+| OPT_exp_x_one
+| OPT_exp_one_x
+| OPT_exp_zero_x
+| OPT_exp_two_x
+| OPT_gt_zero_x
+| OPT_gt_x_x
+| OPT_lt_x_zero
+| OPT_lt_x_x
+| OPT_eq_x_x
+| OPT_iszero_sub
+| OPT_iszero_lt
+| OPT_iszero_xor
+| OPT_iszero2_gt
+| OPT_iszero2_lt
+| OPT_iszero2_eq
+| OPT_xor_x_x
+| OPT_xor_zero
+| OPT_xor_xor
+| OPT_or_or
+| OPT_or_and
+| OPT_and_or
+| OPT_and_not
+| OPT_or_not
+| OPT_or_x_x
+| OPT_and_x_x
+| OPT_or_zero
+| OPT_or_ffff
+| OPT_and_ffff
+| OPT_and_coinbase
+| OPT_balance_address
+| OPT_slt_x_x
+| OPT_sgt_x_x
+.
+
+
+Definition list_opt_steps := list available_optimization_step.
+
+Definition get_optimization_step (tag: available_optimization_step) : opt_entry :=
+match tag with 
+| OPT_eval => OpEntry optimize_eval_sbinding optimize_eval_sbinding_snd
+| OPT_add_zero => OpEntry optimize_add_zero_sbinding optimize_add_zero_sbinding_snd
+| OPT_not_not => OpEntry optimize_not_not_sbinding optimize_not_not_sbinding_snd
+| OPT_and_and => OpEntry optimize_and_and_sbinding optimize_and_and_sbinding_snd
+| OPT_and_origin => OpEntry optimize_and_origin_sbinding optimize_and_origin_sbinding_snd
+| OPT_mul_shl => OpEntry optimize_mul_shl_sbinding optimize_mul_shl_sbinding_snd
+| OPT_div_shl => OpEntry optimize_div_shl_sbinding optimize_div_shl_sbinding_snd
+| OPT_shr_zero_x => OpEntry optimize_shr_zero_x_sbinding optimize_shr_zero_x_sbinding_snd
+| OPT_shr_x_zero => OpEntry optimize_shr_x_zero_sbinding optimize_shr_x_zero_sbinding_snd
+| OPT_eq_zero => OpEntry optimize_eq_zero_sbinding optimize_eq_zero_sbinding_snd
+| OPT_sub_x_x => OpEntry optimize_sub_x_x_sbinding optimize_sub_x_x_sbinding_snd
+| OPT_and_zero => OpEntry optimize_and_zero_sbinding optimize_and_zero_sbinding_snd
+| OPT_div_one => OpEntry optimize_div_one_sbinding optimize_div_one_sbinding_snd
+| OPT_lt_x_one => OpEntry optimize_lt_x_one_sbinding optimize_lt_x_one_sbinding_snd
+| OPT_gt_one_x => OpEntry optimize_gt_one_x_sbinding optimize_gt_one_x_sbinding_snd
+| OPT_and_address => OpEntry optimize_and_address_sbinding optimize_and_address_sbinding_snd
+| OPT_mul_one => OpEntry optimize_mul_one_sbinding optimize_mul_one_sbinding_snd
+| OPT_iszero_gt => OpEntry optimize_iszero_gt_sbinding optimize_iszero_gt_sbinding_snd
+| OPT_eq_iszero => OpEntry optimize_eq_iszero_sbinding optimize_eq_iszero_sbinding_snd
+| OPT_and_caller => OpEntry optimize_and_caller_sbinding optimize_and_caller_sbinding_snd
+| OPT_iszero3 => OpEntry optimize_iszero3_sbinding optimize_iszero3_sbinding_snd
+| OPT_add_sub => OpEntry optimize_add_sub_sbinding optimize_add_sub_sbinding_snd
+| OPT_shl_zero_x => OpEntry optimize_shl_zero_x_sbinding optimize_shl_zero_x_sbinding_snd
+| OPT_sub_zero => OpEntry optimize_sub_zero_sbinding optimize_sub_zero_sbinding_snd
+| OPT_shl_x_zero => OpEntry optimize_shl_x_zero_sbinding optimize_shl_x_zero_sbinding_snd
+| OPT_mul_zero => OpEntry optimize_mul_zero_sbinding optimize_mul_zero_sbinding_snd
+| OPT_div_x_x => OpEntry optimize_div_x_x_sbinding optimize_div_x_x_sbinding_snd
+| OPT_div_zero => OpEntry optimize_div_zero_sbinding optimize_div_zero_sbinding_snd
+| OPT_mod_one => OpEntry optimize_mod_one_sbinding optimize_mod_one_sbinding_snd
+| OPT_mod_zero => OpEntry optimize_mod_zero_sbinding optimize_mod_zero_sbinding_snd
+| OPT_mod_x_x => OpEntry optimize_mod_x_x_sbinding optimize_mod_x_x_sbinding_snd
+| OPT_exp_x_zero => OpEntry optimize_exp_x_zero_sbinding optimize_exp_x_zero_sbinding_snd
+| OPT_exp_x_one => OpEntry optimize_exp_x_one_sbinding optimize_exp_x_one_sbinding_snd
+| OPT_exp_one_x => OpEntry optimize_exp_one_x_sbinding optimize_exp_one_x_sbinding_snd
+| OPT_exp_zero_x => OpEntry optimize_exp_zero_x_sbinding optimize_exp_zero_x_sbinding_snd
+| OPT_exp_two_x => OpEntry optimize_exp_two_x_sbinding optimize_exp_two_x_sbinding_snd
+| OPT_gt_zero_x => OpEntry optimize_gt_zero_x_sbinding optimize_gt_zero_x_sbinding_snd
+| OPT_gt_x_x => OpEntry optimize_gt_x_x_sbinding optimize_gt_x_x_sbinding_snd
+| OPT_lt_x_zero => OpEntry optimize_lt_x_zero_sbinding optimize_lt_x_zero_sbinding_snd
+| OPT_lt_x_x => OpEntry optimize_lt_x_x_sbinding optimize_lt_x_x_sbinding_snd
+| OPT_eq_x_x => OpEntry optimize_eq_x_x_sbinding optimize_eq_x_x_sbinding_snd
+| OPT_iszero_sub => OpEntry optimize_iszero_sub_sbinding optimize_iszero_sub_sbinding_snd
+| OPT_iszero_lt => OpEntry optimize_iszero_lt_sbinding optimize_iszero_lt_sbinding_snd
+| OPT_iszero_xor => OpEntry optimize_iszero_xor_sbinding optimize_iszero_xor_sbinding_snd
+| OPT_iszero2_gt => OpEntry optimize_iszero2_gt_sbinding optimize_iszero2_gt_sbinding_snd
+| OPT_iszero2_lt => OpEntry optimize_iszero2_lt_sbinding optimize_iszero2_lt_sbinding_snd
+| OPT_iszero2_eq => OpEntry optimize_iszero2_eq_sbinding optimize_iszero2_eq_sbinding_snd
+| OPT_xor_x_x => OpEntry optimize_xor_x_x_sbinding optimize_xor_x_x_sbinding_snd
+| OPT_xor_zero => OpEntry optimize_xor_zero_sbinding optimize_xor_zero_sbinding_snd
+| OPT_xor_xor => OpEntry optimize_xor_xor_sbinding optimize_xor_xor_sbinding_snd
+| OPT_or_or => OpEntry optimize_or_or_sbinding optimize_or_or_sbinding_snd
+| OPT_or_and => OpEntry optimize_or_and_sbinding optimize_or_and_sbinding_snd
+| OPT_and_or => OpEntry optimize_and_or_sbinding optimize_and_or_sbinding_snd
+| OPT_and_not => OpEntry optimize_and_not_sbinding optimize_and_not_sbinding_snd
+| OPT_or_not => OpEntry optimize_or_not_sbinding optimize_or_not_sbinding_snd
+| OPT_or_x_x => OpEntry optimize_or_x_x_sbinding optimize_or_x_x_sbinding_snd
+| OPT_and_x_x => OpEntry optimize_and_x_x_sbinding optimize_and_x_x_sbinding_snd
+| OPT_or_zero => OpEntry optimize_or_zero_sbinding optimize_or_zero_sbinding_snd
+| OPT_or_ffff => OpEntry optimize_or_ffff_sbinding optimize_or_ffff_sbinding_snd
+| OPT_and_ffff => OpEntry optimize_and_ffff_sbinding optimize_and_ffff_sbinding_snd
+| OPT_and_coinbase => OpEntry optimize_and_coinbase_sbinding optimize_and_coinbase_sbinding_snd
+| OPT_balance_address => OpEntry optimize_balance_address_sbinding optimize_balance_address_sbinding_snd
+| OPT_slt_x_x => OpEntry optimize_slt_x_x_sbinding optimize_slt_x_x_sbinding_snd
+| OPT_sgt_x_x => OpEntry optimize_sgt_x_x_sbinding optimize_sgt_x_x_sbinding_snd
+end.
+
+Definition all_optimization_steps := 
+  [OPT_eval; 
+   OPT_add_zero; 
+   OPT_not_not; 
+   OPT_and_and;    
+   OPT_and_origin; 
+   OPT_div_shl;
+   OPT_mul_shl;
+   OPT_shr_zero_x; 
+   OPT_shr_x_zero; 
+   OPT_eq_zero; 
+   OPT_sub_x_x; 
+   OPT_and_zero; 
+   OPT_div_one; 
+   OPT_lt_x_one; 
+   OPT_gt_one_x; 
+   OPT_and_address; 
+   OPT_mul_one; 
+   OPT_iszero_gt; 
+   OPT_eq_iszero;
+   OPT_and_caller;
+   OPT_iszero3;
+   OPT_add_sub;
+   OPT_shl_zero_x;
+   OPT_sub_zero;
+   OPT_shl_x_zero;
+   OPT_mul_zero;
+   OPT_div_x_x;  (* TODO:  useless: checking X <> 0 requires X to be a value
+                           so DIV(X,X) contains constants and can be avaluated
+                           by the "eval" optimization *)
+   OPT_div_zero;
+   OPT_mod_one;
+   OPT_mod_zero;
+   OPT_mod_x_x;
+   OPT_exp_x_zero;
+   OPT_exp_x_one;
+   OPT_exp_one_x;
+   OPT_exp_zero_x;
+   OPT_exp_two_x;
+   OPT_gt_zero_x;
+   OPT_gt_x_x;
+   OPT_lt_x_zero;
+   OPT_lt_x_x;
+   OPT_eq_x_x;
+   OPT_iszero_sub;
+   OPT_iszero_lt;
+   OPT_iszero_xor;
+   OPT_iszero2_gt;
+   OPT_iszero2_lt;
+   OPT_iszero2_eq;
+   OPT_xor_x_x;
+   OPT_xor_zero;
+   OPT_xor_xor;
+   OPT_or_or;
+   OPT_or_and;
+   OPT_and_or;
+   OPT_and_not;
+   OPT_or_not;
+   OPT_or_x_x;
+   OPT_and_x_x;
+   OPT_or_zero;
+   OPT_or_ffff;
+   OPT_and_ffff;
+   OPT_and_coinbase;
+   OPT_balance_address;
+   OPT_slt_x_x;
+   OPT_sgt_x_x
+].
+
+Definition all_optimization_steps' := 
+  [OPT_div_shl;
+   OPT_mul_shl;
+   OPT_eval; 
+   OPT_add_zero; 
+   OPT_not_not; 
+   OPT_and_and;    
+   OPT_and_origin; 
+   OPT_shr_zero_x; 
+   OPT_shr_x_zero; 
+   OPT_eq_zero; 
+   OPT_sub_x_x; 
+   OPT_and_zero; 
+   OPT_div_one; 
+   OPT_lt_x_one; 
+   OPT_gt_one_x; 
+   OPT_and_address; 
+   OPT_mul_one; 
+   OPT_iszero_gt; 
+   OPT_eq_iszero;
+   OPT_and_caller;
+   OPT_iszero3;
+   OPT_add_sub;
+   OPT_shl_zero_x;
+   OPT_sub_zero;
+   OPT_shl_x_zero;
+   OPT_mul_zero;
+   OPT_div_x_x;  (* TODO:  useless: checking X <> 0 requires X to be a value
+                           so DIV(X,X) contains constants and can be avaluated
+                           by the "eval" optimization *)
+   OPT_div_zero;
+   OPT_mod_one;
+   OPT_mod_zero;
+   OPT_mod_x_x;
+   OPT_exp_x_zero;
+   OPT_exp_x_one;
+   OPT_exp_one_x;
+   OPT_exp_zero_x;
+   OPT_exp_two_x;
+   OPT_gt_zero_x;
+   OPT_gt_x_x;
+   OPT_lt_x_zero;
+   OPT_lt_x_x;
+   OPT_eq_x_x;
+   OPT_iszero_sub;
+   OPT_iszero_lt;
+   OPT_iszero_xor;
+   OPT_iszero2_gt;
+   OPT_iszero2_lt;
+   OPT_iszero2_eq;
+   OPT_xor_x_x;
+   OPT_xor_zero;
+   OPT_xor_xor;
+   OPT_or_or;
+   OPT_or_and;
+   OPT_and_or;
+   OPT_and_not;
+   OPT_or_not;
+   OPT_or_x_x;
+   OPT_and_x_x;
+   OPT_or_zero;
+   OPT_or_ffff;
+   OPT_and_ffff;
+   OPT_and_coinbase;
+   OPT_balance_address;
+   OPT_slt_x_x;
+   OPT_sgt_x_x   
+].
+
+  
+Fixpoint get_pipeline (l: list_opt_steps) : opt_pipeline :=
+match l with 
+| nil => nil
+| tag::r => (get_optimization_step tag)::(get_pipeline r)
+end.
+
+
+Definition checker_type := constraints -> sstate -> block -> block -> bool.
+
+Definition evm_eq_block_chkr'
+  (memory_updater: smemory_updater_ext_type) 
+  (storage_updater: sstorage_updater_ext_type)
+  (mload_solver: mload_solver_ext_type) 
+  (sload_solver: sload_solver_ext_type)
+  (sstack_value_cmp_ext: sstack_val_cmp_ext_2_t)
+  (smemory_cmp_ext: smemory_cmp_ext_t)
+  (sstorage_cmp_ext: sstorage_cmp_ext_t)
+  (sha3_cmp_ext: sha3_cmp_ext_t)
+  (opt_pipeline: opt_pipeline)
+  (opt_step_rep: nat)
+  (opt_pipeline_rep: nat)
+  (***)
+  (ctx : constraints)
+  (init_sst : sstate) 
+  (opt_p p: block)
+  : bool :=
+  if (chk_valid_sstate init_sst evm_stack_opm) && (chk_is_sat ctx) then
+    let sstack_value_cmp_1 := sstack_value_cmp_ext smemory_cmp_ext sstorage_cmp_ext sha3_cmp_ext in
+    let memory_updater' := memory_updater sstack_value_cmp_1 in
+    let storage_updater' := storage_updater sstack_value_cmp_1 in
+    let mload_solver' := mload_solver sstack_value_cmp_1 in
+    let sload_solver' := sload_solver sstack_value_cmp_1 in
+    
+    match evm_exec_block_s memory_updater' storage_updater' mload_solver' sload_solver' opt_p ctx init_sst evm_stack_opm with
+    | None => false
+    | Some sst_opt => 
+        match evm_exec_block_s memory_updater' storage_updater' mload_solver' sload_solver' p ctx init_sst evm_stack_opm with 
+        | None => false
+        | Some sst_p => (* Builds optimization *)
+            let maxid := S (max (get_maxidx_smap (get_smap_sst sst_opt)) (get_maxidx_smap (get_smap_sst sst_p))) in
+            let sstack_value_cmp := sstack_value_cmp_1 maxid in
+            let opt := apply_opt_n_times_pipeline_k opt_pipeline 
+                         sstack_value_cmp opt_step_rep 
+                         opt_pipeline_rep in
+            (* opt is sound if sstack_value_cmp is "safe_sstack_val_cmp" *)
+            
+            let (sst_opt', _) := opt ctx sst_opt in 
+            let (sst_p',   _) := opt ctx sst_p in
+            let smemory_cmp := smemory_cmp_ext sstack_value_cmp in
+            let sstorage_cmp := sstorage_cmp_ext sstack_value_cmp in
+            sstate_cmp sstack_value_cmp smemory_cmp sstorage_cmp ctx sst_p' sst_opt' evm_stack_opm
+        end
+    end
+  else false.
+  
+
+Definition evm_eq_block_chkr_lazy
+  (memory_updater_tag: available_smemory_updaters) 
+  (storage_updater_tag: available_sstorage_updaters)
+  (mload_solver_tag: available_mload_solvers) 
+  (sload_solver_tag: available_sload_solvers)
+  (sstack_value_cmp_tag: available_sstack_val_cmp)
+  (memory_cmp_tag: available_memory_cmp)
+  (storage_cmp_tag: available_storage_cmp)
+  (sha3_cmp_tag: available_sha3_cmp)
+  
+  (*(opt: optim)*)
+  (optimization_steps: list_opt_steps)
+  (opt_step_rep: nat)
+  (opt_pipeline_rep: nat) :=
+  
+  match get_smemory_updater memory_updater_tag with
+  | SMemUpdater memory_updater _ =>
+      match get_sstorage_updater storage_updater_tag with
+      | SStrgUpdater storage_updater _ =>
+          match get_mload_solver mload_solver_tag with
+          | MLoadSolver mload_solver _ =>
+             match get_sload_solver sload_solver_tag with
+             | SLoadSolver sload_solver _ =>
+                 match get_sstack_val_cmp sstack_value_cmp_tag with
+                 | SStackValCmp sstack_val_cmp _ _ =>
+                     match get_memory_cmp memory_cmp_tag with
+                     | SMemCmp memory_cmp _ =>
+                         match get_storage_cmp storage_cmp_tag with 
+                         | SStrgCmp storage_cmp _ =>
+                             match get_sha3_cmp sha3_cmp_tag with
+                               | SHA3Cmp sha3_cmp _ => 
+                                   match get_pipeline optimization_steps with
+                                   | opt_pipeline =>
+                                       fun (ctx : constraints) (init_sst : sstate) (opt_p p: block) =>
+                                         evm_eq_block_chkr' memory_updater storage_updater mload_solver sload_solver sstack_val_cmp memory_cmp storage_cmp sha3_cmp opt_pipeline opt_step_rep opt_pipeline_rep ctx init_sst opt_p p
+                                   end
+                             end
+                         end
+                     end
+                 end
+             end
+          end
+      end
+  end.
+
+
+
+Definition evm_eq_block_chkr
+  (memory_updater_tag: available_smemory_updaters) 
+  (storage_updater_tag: available_sstorage_updaters)
+  (mload_solver_tag: available_mload_solvers) 
+  (sload_solver_tag: available_sload_solvers)
+  (sstack_value_cmp_tag: available_sstack_val_cmp)
+  (memory_cmp_tag: available_memory_cmp)
+  (storage_cmp_tag: available_storage_cmp)
+  (sha3_cmp_tag: available_sha3_cmp)
+  
+  (opt_pipeline: list_opt_steps)
+  (opt_step_rep: nat)
+  (opt_pipeline_rep: nat)
+  
+  (ctx : constraints)
+  (init_sst : sstate) 
+  (opt_p p: block) :=
+  let chkr := evm_eq_block_chkr_lazy memory_updater_tag storage_updater_tag mload_solver_tag sload_solver_tag sstack_value_cmp_tag memory_cmp_tag storage_cmp_tag sha3_cmp_tag opt_pipeline opt_step_rep opt_pipeline_rep in
+  chkr ctx init_sst opt_p p.
+
+
+
+
+Definition sem_eq_blocks (p1 p2: block) (ctx: constraints) (sst: sstate) : Prop :=
+  forall (mem: memory) (strg: storage) (exts: externals) (in_st: state) (model: assignment),
+    is_model ctx model = true ->
+    st_is_instance_of_sst mem strg exts in_st model sst evm_stack_opm ->
+    exists (out_st1 out_st2 : state),
+      evm_exec_block_c p1 in_st evm_stack_opm = Some out_st1 /\
+        evm_exec_block_c p2 in_st evm_stack_opm = Some out_st2 /\
+        eq_execution_states out_st1 out_st2.
+
+Definition eq_block_chkr_snd (chkr : checker_type) : Prop :=
+forall (p1 p2: block) (ctx: constraints) (sst: sstate),
+  chkr ctx sst p1 p2 = true
+  -> sem_eq_blocks p1 p2 ctx sst.
+
+
+End BlockEquivChecker.
+
