block_equiv_checker_soundness.v
@@ -1,0 +1,404 @@
+Require Import Bool.
+Require Import List.
+
+Require Import FORVES2.program.
+Import Program.
+
+Require Import FORVES2.stack_operation_instructions.
+Import StackOpInstrs.
+
+Require Import FORVES2.execution_state.
+Import ExecutionState.
+
+Require Import FORVES2.execution_state_facts.
+Import ExecutionStateFacts.
+
+Require Import FORVES2.concrete_interpreter.
+Import ConcreteInterpreter.
+
+Require Import FORVES2.optimizations_def.
+Import Optimizations_Def.
+
+Require Import FORVES2.symbolic_execution.
+Import SymbolicExecution.
+
+Require Import FORVES2.storage_ops_solvers.
+Import StorageOpsSolvers.
+
+Require Import FORVES2.storage_ops_solvers_impl.
+Import StorageOpsSolversImpl.
+
+Require Import FORVES2.memory_ops_solvers.
+Import MemoryOpsSolvers.
+
+Require Import FORVES2.memory_ops_solvers_impl.
+Import MemoryOpsSolversImpl.
+
+Require Import FORVES2.symbolic_state_cmp.
+Import SymbolicStateCmp.
+
+Require Import FORVES2.valid_symbolic_state.
+Import ValidSymbolicState.
+
+Require Import FORVES2.symbolic_execution_soundness.
+Import SymbolicExecutionSoundness.
+
+Require Import FORVES2.symbolic_state_eval.
+Import SymbolicStateEval.
+
+Require Import FORVES2.symbolic_state.
+Import SymbolicState.
+
+Require Import FORVES2.symbolic_state_cmp_impl.
+Import SymbolicStateCmpImpl.
+
+Require Import FORVES2.sstack_val_cmp_impl.
+Import SStackValCmpImpl.
+
+Require Import FORVES2.sstack_val_cmp_impl_soundness.
+Import SStackValCmpImplSoundness.
+
+Require Import FORVES2.sha3_cmp_impl.
+Import SHA3CmpImpl.
+
+Require Import FORVES2.sha3_cmp_impl_soundness.
+Import SHA3CmpImplSoundness.
+
+Require Import FORVES2.storage_cmp_impl.
+Import StorageCmpImpl.
+
+Require Import FORVES2.storage_cmp_impl_soundness.
+Import StorageCmpImplSoundness.
+
+
+Require Import FORVES2.memory_cmp_impl.
+Import MemoryCmpImpl.
+
+Require Import FORVES2.memory_cmp_impl_soundness.
+Import MemoryCmpImplSoundness.
+
+Require Import FORVES2.storage_ops_solvers_impl.
+Import StorageOpsSolversImpl.
+
+Require Import FORVES2.storage_ops_solvers_impl_soundness.
+Import StorageOpsSolversImplSoundness.
+
+Require Import FORVES2.memory_ops_solvers_impl.
+Import MemoryOpsSolversImpl.
+
+Require Import FORVES2.memory_ops_solvers_impl_soundness.
+Import MemoryOpsSolversImplSoundness.
+
+Require Import FORVES2.symbolic_state_cmp_impl_soundness.
+Import SymbolicStateCmpImplSoundness.
+
+Require Import FORVES2.misc.
+Import Misc.
+
+Require Import FORVES2.block_equiv_checker.
+Import BlockEquivChecker.
+
+
+Require Import FORVES2.constraints.
+Import Constraints.
+
+From Coq Require Import Lists.List. Import ListNotations.
+
+Module BlockEquivCheckerSoundness.
+
+Lemma evm_eq_block_chkr'_snd: forall
+    (memory_updater: smemory_updater_ext_type) 
+    (storage_updater: sstorage_updater_ext_type)
+    (mload_solver: mload_solver_ext_type) 
+    (sload_solver: sload_solver_ext_type)
+    (sstack_value_cmp_ext: sstack_val_cmp_ext_2_t)
+    (smemory_cmp_ext: smemory_cmp_ext_t)
+    (sstorage_cmp_ext: sstorage_cmp_ext_t)
+    (sha3_cmp_ext: sha3_cmp_ext_t)
+    (opt_pipeline: opt_pipeline)
+    (opt_step_rep: nat)
+    (opt_pipeline_rep: nat),
+    smemory_updater_ext_snd memory_updater ->
+    sstorage_updater_ext_snd storage_updater ->
+    mload_solver_ext_snd mload_solver ->
+    sload_solver_ext_snd sload_solver ->
+    sstack_val_cmp_fail_for_d_eq_0 sstack_value_cmp_ext ->
+    safe_smemory_cmp_ext_wrt_sstack_value_cmp smemory_cmp_ext ->
+    safe_sstorage_cmp_ext_wrt_sstack_value_cmp sstorage_cmp_ext ->
+    safe_sha3_cmp_ext_wrt_sstack_value_cmp sha3_cmp_ext ->
+    safe_sstack_value_cmp_wrt_others sstack_value_cmp_ext ->
+
+    eq_block_chkr_snd (evm_eq_block_chkr' memory_updater storage_updater mload_solver sload_solver sstack_value_cmp_ext smemory_cmp_ext sstorage_cmp_ext sha3_cmp_ext opt_pipeline opt_step_rep opt_pipeline_rep).
+Proof.
+  intros memory_updater storage_updater mload_solver sload_solver sstack_value_cmp_ext smemory_cmp_ext sstorage_cmp_ext sha3_cmp_ext opt_pipeline opt_step_rep opt_pipeline_rep H_smemory_updater_ext_snd H_sstorage_updater_ext_snd H_mload_solver_ext_snd H_sload_solver_ext_snd H_sstack_val_cmp_fail_for_d_eq_0 H_safe_smemory_cmp_ext_wrt_sstack_value_cmp H_safe_sstorage_cmp_ext_wrt_sstack_value_cmp H_safe_sha3_cmp_ext_wrt_sstack_value_cmp H_safe_sstack_value_cmp_wrt_others.
+
+  (* combining the comparators results in a sound one *)
+  pose proof (safe_all_cmp smemory_cmp_ext sstorage_cmp_ext sha3_cmp_ext sstack_value_cmp_ext H_sstack_val_cmp_fail_for_d_eq_0 H_safe_smemory_cmp_ext_wrt_sstack_value_cmp H_safe_sstorage_cmp_ext_wrt_sstack_value_cmp H_safe_sha3_cmp_ext_wrt_sstack_value_cmp H_safe_sstack_value_cmp_wrt_others) as H_safe_all_cmp.
+
+  unfold eq_block_chkr_snd.
+  intros p1 p2 ctx sst H_evm_eq_block_chkr'.
+
+  unfold evm_eq_block_chkr' in H_evm_eq_block_chkr'.
+
+
+  destruct (chk_valid_sstate sst evm_stack_opm && chk_is_sat ctx)%bool eqn:E_valid_and_sat; try discriminate.
+  apply andb_prop in E_valid_and_sat.
+  destruct E_valid_and_sat as [H_valid_sst_b H_is_sat_b].
+  
+  pose proof (chk_valid_sstate_snd sst evm_stack_opm H_valid_sst_b) as H_valid_sst.
+  pose proof (chk_is_sat_snd ctx H_is_sat_b) as H_is_sat.
+
+  remember (sstack_value_cmp_ext smemory_cmp_ext sstorage_cmp_ext sha3_cmp_ext) as sstack_value_cmp_1.
+  remember (memory_updater sstack_value_cmp_1) as memory_updater'.
+
+  remember (storage_updater sstack_value_cmp_1) as storage_updater'.
+  remember (mload_solver sstack_value_cmp_1) as mload_solver'.
+  remember (sload_solver sstack_value_cmp_1) as sload_solver'.
+
+
+  destruct (evm_exec_block_s memory_updater' storage_updater' mload_solver' sload_solver' p1 ctx sst evm_stack_opm) as [sst_opt|] eqn:E_sym_exec_p1; try discriminate.
+
+  destruct (evm_exec_block_s memory_updater' storage_updater' mload_solver' sload_solver' p2 ctx sst evm_stack_opm) as [sst_p|] eqn:E_sym_exec_p2; try discriminate.
+
+  remember (S (max (get_maxidx_smap (get_smap_sst sst_opt)) (get_maxidx_smap (get_smap_sst sst_p)))) as maxid.
+  remember (sstack_value_cmp_1 maxid) as sstack_value_cmp.
+  remember (apply_opt_n_times_pipeline_k opt_pipeline sstack_value_cmp opt_step_rep opt_pipeline_rep) as opt.
+
+  destruct (opt ctx sst_opt) as [sst_opt' aux_bool_opt1] eqn:H_sst_opt_apply_op.
+  destruct (opt ctx sst_p) as [sst_p' aux_bool_opt2] eqn:H_sst_p_apply_op.
+
+  remember (smemory_cmp_ext sstack_value_cmp) as smemory_cmp.
+  remember (sstorage_cmp_ext sstack_value_cmp) as sstorage_cmp.
+
+  pose proof (safe_ext_all_cmp smemory_cmp_ext sstorage_cmp_ext sha3_cmp_ext sstack_value_cmp_ext H_sstack_val_cmp_fail_for_d_eq_0 H_safe_smemory_cmp_ext_wrt_sstack_value_cmp H_safe_sstorage_cmp_ext_wrt_sstack_value_cmp H_safe_sha3_cmp_ext_wrt_sstack_value_cmp H_safe_sstack_value_cmp_wrt_others) as [H_sstack_value_cmp_ext [H_smemory_cmp_ext [H_sstorage_cmp_ext H_sha3_cmp_ext ]]].
+
+
+  assert (H_sstack_value_cmp_ext_1: forall d, safe_sstack_val_cmp_ext_1_d sstack_value_cmp_1 d).
+  (* proof of assert *)
+  rewrite Heqsstack_value_cmp_1.
+  intros.
+  apply safe_ext_2_implies_safe_ext_1.
+  apply H_sstack_value_cmp_ext.
+  (* end of proof of assert *)
+  
+  assert (H_sstack_value_cmp_ext_1': safe_sstack_val_cmp_ext_1 sstack_value_cmp_1).
+  (* proof of assert *)
+  unfold safe_sstack_val_cmp_ext_1.
+  apply H_sstack_value_cmp_ext_1.
+  (* end of proof of assert *)
+
+  
+  assert (H_memory_updater'_snd: smemory_updater_snd memory_updater').
+  (* proof of assert *)
+  unfold safe_sstack_val_cmp_ext_2 in H_sstack_value_cmp_ext.
+  unfold smemory_updater_ext_snd in H_smemory_updater_ext_snd.
+  pose proof (H_smemory_updater_ext_snd sstack_value_cmp_1 H_sstack_value_cmp_ext_1') as H_smemory_updater_ext_snd'.
+  rewrite <- Heqmemory_updater' in H_smemory_updater_ext_snd'.
+  apply H_smemory_updater_ext_snd'.
+  (* end of proof of assert *)
+
+
+  assert (H_storage_updater'_snd: sstorage_updater_snd storage_updater').
+  (* proof of assert *)
+  unfold safe_sstack_val_cmp_ext_2 in H_sstack_value_cmp_ext.
+  unfold sstorage_updater_ext_snd in H_sstorage_updater_ext_snd.
+  pose proof (H_sstorage_updater_ext_snd sstack_value_cmp_1 H_sstack_value_cmp_ext_1') as H_sstorage_updater_ext_snd'.
+  rewrite <- Heqstorage_updater' in H_sstorage_updater_ext_snd'.
+  apply H_sstorage_updater_ext_snd'.
+  (* end of proof of assert *)
+
+  assert (H_mload_solver'_snd: mload_solver_snd mload_solver').
+  (* proof of assert *)
+  unfold safe_sstack_val_cmp_ext_2 in H_sstack_value_cmp_ext.
+  unfold mload_solver_ext_snd in H_mload_solver_ext_snd.
+  pose proof (H_mload_solver_ext_snd sstack_value_cmp_1 H_sstack_value_cmp_ext_1') as H_mload_solver_ext_snd'.
+  rewrite <- Heqmload_solver' in H_mload_solver_ext_snd'.
+  apply H_mload_solver_ext_snd'.
+  (* end of proof of assert *)
+
+  assert (H_sload_solver'_snd: sload_solver_snd sload_solver').
+  (* proof of assert *)
+  unfold safe_sstack_val_cmp_ext_2 in H_sstack_value_cmp_ext.
+  unfold sload_solver_ext_snd in H_sload_solver_ext_snd.
+  pose proof (H_sload_solver_ext_snd sstack_value_cmp_1 H_sstack_value_cmp_ext_1') as H_sload_solver_ext_snd'.
+  rewrite <- Heqsload_solver' in H_sload_solver_ext_snd'.
+  apply H_sload_solver_ext_snd'.
+  (* end of proof of assert *)
+
+  (* soundness of symbolic execution of p1 *)
+  pose proof (symbolic_exec_snd memory_updater' storage_updater' mload_solver' sload_solver' p1 ctx sst sst_opt evm_stack_opm H_is_sat H_valid_sst H_memory_updater'_snd H_storage_updater'_snd H_mload_solver'_snd H_sload_solver'_snd E_sym_exec_p1) as [H_sym_exc_snd_p1_1 H_sym_exc_snd_p1_2].
+
+  (* soundness of symbolic execution of p2 *)
+  pose proof (symbolic_exec_snd memory_updater' storage_updater' mload_solver' sload_solver' p2 ctx sst sst_p evm_stack_opm H_is_sat H_valid_sst H_memory_updater'_snd H_storage_updater'_snd H_mload_solver'_snd H_sload_solver'_snd E_sym_exec_p2) as [H_sym_exc_snd_p2_1  H_sym_exc_snd_p2_2].
+
+  assert (H_safe_sstack_value_cmp: safe_sstack_val_cmp sstack_value_cmp).
+  (* proof of assert *)
+  unfold  safe_sstack_val_cmp_ext_1 in H_sstack_value_cmp_ext_1'.
+  pose proof (H_sstack_value_cmp_ext_1 maxid) as H_sstack_value_cmp_ext_1'_maxid.
+  unfold safe_sstack_val_cmp_ext_1_d in H_sstack_value_cmp_ext_1'_maxid.
+  pose proof (H_sstack_value_cmp_ext_1'_maxid maxid (PeanoNat.Nat.le_refl maxid)) as H_sstack_value_cmp_ext_1'_maxid.
+  rewrite Heqsstack_value_cmp.
+  apply H_sstack_value_cmp_ext_1'_maxid.
+  (* end of proof of assert *)
+
+  (* opt that is generated by the pipeline is sound *)
+  pose proof (apply_opt_n_times_pipeline_k_snd opt_pipeline sstack_value_cmp opt_step_rep opt_pipeline_rep H_safe_sstack_value_cmp) as H_safe_opt.
+  rewrite <- Heqopt in H_safe_opt.
+
+  assert (H_safe_smemory_cmp: safe_smemory_cmp smemory_cmp).
+  (* proof of assert *)
+  rewrite <- Heqsstack_value_cmp_1 in H_smemory_cmp_ext.
+  unfold safe_smemory_cmp_ext in H_smemory_cmp_ext.
+  pose proof (H_smemory_cmp_ext maxid) as H_smemory_cmp_ext.
+  unfold safe_smemory_cmp_ext_d in H_smemory_cmp_ext.
+  pose proof (H_smemory_cmp_ext maxid (PeanoNat.Nat.le_refl maxid)) as H_smemory_cmp_ext_maxid.
+  rewrite <- Heqsstack_value_cmp in H_smemory_cmp_ext_maxid.
+  rewrite <- Heqsmemory_cmp in H_smemory_cmp_ext_maxid.
+  apply H_smemory_cmp_ext_maxid.
+  (* end of proof of assert *)
+  
+  assert (H_safe_sstorage_cmp: safe_sstorage_cmp sstorage_cmp).
+  (* proof of assert *)
+  rewrite <- Heqsstack_value_cmp_1 in H_sstorage_cmp_ext.
+  unfold safe_sstorage_cmp_ext in H_sstorage_cmp_ext.
+  pose proof (H_sstorage_cmp_ext maxid) as H_sstorage_cmp_ext.
+  unfold safe_sstorage_cmp_ext_d in H_sstorage_cmp_ext.
+  pose proof (H_sstorage_cmp_ext maxid (PeanoNat.Nat.le_refl maxid)) as H_sstorage_cmp_ext_maxid.
+  rewrite <- Heqsstack_value_cmp in H_sstorage_cmp_ext_maxid.
+  rewrite <- Heqsstorage_cmp in H_sstorage_cmp_ext_maxid.
+  apply H_sstorage_cmp_ext_maxid.
+  (* end of proof of assert *)
+ 
+  pose proof (sstate_cmp_snd sstack_value_cmp smemory_cmp sstorage_cmp H_safe_sstack_value_cmp H_safe_smemory_cmp H_safe_sstorage_cmp) as H_sstate_cmp_snd.
+  
+  unfold sem_eq_blocks.
+  intros mem strg exts in_st model H_is_model H_in_st_is_instance_of_sst.
+
+  pose proof (H_sym_exc_snd_p1_2 mem strg exts in_st model H_is_model H_in_st_is_instance_of_sst) as H_sym_exc_snd_p1_2.
+  destruct H_sym_exc_snd_p1_2 as [st'_1 [H_sym_exc_snd_p1_2_1 H_sym_exc_snd_p1_2_2]].
+  
+  pose proof (H_sym_exc_snd_p2_2  mem strg exts in_st model H_is_model H_in_st_is_instance_of_sst) as H_sym_exc_snd_p2_2.
+  destruct H_sym_exc_snd_p2_2 as [st'_2 [H_sym_exc_snd_p2_2_1 H_sym_exc_snd_p2_2_2]].
+
+  exists st'_1. exists st'_2.
+  split; try split; try apply H_sym_exc_snd_p1_2_1; try apply H_sym_exc_snd_p2_2_1.
+
+  unfold optim_snd in H_safe_opt.
+
+  
+  pose proof (H_safe_opt ctx sst_opt sst_opt' aux_bool_opt1 H_is_sat H_sym_exc_snd_p1_1 H_sst_opt_apply_op) as [H_optim_snd_1_1 H_optim_snd_1_2].
+ 
+  pose proof (H_safe_opt ctx sst_p sst_p' aux_bool_opt2 H_is_sat H_sym_exc_snd_p2_1 H_sst_p_apply_op) as [H_optim_snd_2_1 H_optim_snd_2_2].
+ 
+  unfold st_is_instance_of_sst in H_sym_exc_snd_p1_2_2.
+  destruct H_sym_exc_snd_p1_2_2 as [st1' [H_sym_exc_snd_p1_2_2_0 H_sym_exc_snd_p1_2_2_1]].
+
+
+  unfold eq_execution_states in H_sym_exc_snd_p1_2_2_1.
+
+  
+  unfold st_is_instance_of_sst in H_sym_exc_snd_p2_2_2.
+  destruct H_sym_exc_snd_p2_2_2 as [st2' [H_sym_exc_snd_p2_2_2_0 H_sym_exc_snd_p2_2_2_1]].
+
+  pose proof (H_optim_snd_1_2 model mem strg exts st1' H_is_model H_sym_exc_snd_p1_2_2_0 ) as H_optim_snd_1_2_0.
+  pose proof (H_optim_snd_2_2 model mem strg exts st2' H_is_model H_sym_exc_snd_p2_2_2_0 ) as H_optim_snd_2_2_0.
+
+
+  unfold eq_execution_states in H_sym_exc_snd_p2_2_2_1.
+
+  unfold symbolic_state_cmp_snd in H_sstate_cmp_snd.
+
+  pose proof (H_sstate_cmp_snd ctx sst_p' sst_opt' evm_stack_opm H_is_sat H_optim_snd_2_1 H_optim_snd_1_1 H_evm_eq_block_chkr' mem strg exts model H_is_model) as H_sstate_cmp_snd_1.
+  
+  destruct H_sstate_cmp_snd_1 as [st' [H_sstate_cmp_snd_1_0 H_sstate_cmp_snd_1_1]].
+  
+  rewrite H_sstate_cmp_snd_1_0 in H_optim_snd_2_2_0.
+  rewrite H_sstate_cmp_snd_1_1 in H_optim_snd_1_2_0.
+  rewrite  H_optim_snd_2_2_0 in H_optim_snd_1_2_0.
+  injection H_optim_snd_1_2_0 as H_optim_snd_1_2_0.
+
+  rewrite H_optim_snd_1_2_0 in H_sym_exc_snd_p2_2_2_1.
+  
+  destruct H_sym_exc_snd_p1_2_2_1 as [H_sym_exc_snd_p1_2_2_1_stk [H_sym_exc_snd_p1_2_2_1_mem [H_sym_exc_snd_p1_2_2_1_strg H_sym_exc_snd_p1_2_2_1_exts]]].
+  
+  destruct H_sym_exc_snd_p2_2_2_1 as [H_sym_exc_snd_p2_2_2_1_stk [H_sym_exc_snd_p2_2_2_1_mem [H_sym_exc_snd_p2_2_2_1_strg H_sym_exc_snd_p2_2_2_1_exts]]].
+
+  unfold eq_execution_states.
+
+  repeat split.
+  + unfold eq_stack.
+    unfold eq_stack in H_sym_exc_snd_p1_2_2_1_stk.
+    unfold eq_stack in H_sym_exc_snd_p2_2_2_1_stk.
+    rewrite H_sym_exc_snd_p1_2_2_1_stk.
+    rewrite H_sym_exc_snd_p2_2_2_1_stk.
+    reflexivity.
+  + unfold eq_memory.
+    unfold eq_memory in H_sym_exc_snd_p1_2_2_1_mem.
+    unfold eq_memory in H_sym_exc_snd_p2_2_2_1_mem.
+    intro w.
+    rewrite H_sym_exc_snd_p1_2_2_1_mem.
+    rewrite H_sym_exc_snd_p2_2_2_1_mem.
+    reflexivity.
+  + unfold eq_storage.
+    unfold eq_storage in H_sym_exc_snd_p1_2_2_1_strg.
+    unfold eq_storage in H_sym_exc_snd_p2_2_2_1_strg.
+    intro w.
+    rewrite H_sym_exc_snd_p1_2_2_1_strg.
+    rewrite H_sym_exc_snd_p2_2_2_1_strg.
+    reflexivity.
+  + unfold eq_externals.
+    unfold eq_externals in H_sym_exc_snd_p1_2_2_1_exts.
+    unfold eq_externals in H_sym_exc_snd_p2_2_2_1_exts.
+    rewrite H_sym_exc_snd_p1_2_2_1_exts.
+    rewrite H_sym_exc_snd_p2_2_2_1_exts.
+    reflexivity.
+Qed.
+
+Lemma evm_eq_block_chkr_lazy_snd:
+  forall (memory_updater_tag: available_smemory_updaters) (storage_updater_tag: available_sstorage_updaters) (mload_solver_tag: available_mload_solvers) 
+  (sload_solver_tag: available_sload_solvers) (sstack_value_cmp_tag: available_sstack_val_cmp) (memory_cmp_tag: available_memory_cmp)
+  (storage_cmp_tag: available_storage_cmp) (sha3_cmp_tag: available_sha3_cmp) (optimization_steps: list_opt_steps) (opt_step_rep: nat) (opt_pipeline_rep: nat) (chkr: checker_type),
+    evm_eq_block_chkr_lazy memory_updater_tag storage_updater_tag mload_solver_tag sload_solver_tag sstack_value_cmp_tag memory_cmp_tag storage_cmp_tag sha3_cmp_tag optimization_steps opt_step_rep opt_pipeline_rep = chkr ->
+    eq_block_chkr_snd chkr.
+Proof.
+  intros memory_updater_tag storage_updater_tag mload_solver_tag sload_solver_tag sstack_value_cmp_tag memory_cmp_tag storage_cmp_tag sha3_cmp_tag optimization_steps opt_step_rep opt_pipeline_rep chkr H_chkr.
+
+  unfold evm_eq_block_chkr_lazy in H_chkr.
+  destruct (get_smemory_updater memory_updater_tag) as [smemory_updater H_smemory_updater_snd].
+  destruct (get_sstorage_updater storage_updater_tag) as [sstorage_updater H_sstorage_updater_snd].
+  destruct (get_mload_solver mload_solver_tag) as [mload_solver H_mload_solver_snd].
+  destruct (get_sload_solver sload_solver_tag) as [sload_solver H_sload_solver_snd].
+  destruct (get_sstack_val_cmp sstack_value_cmp_tag) as [sstack_value_cmp H_sstack_value_cmp_snd  H_sstack_value_cmp_snd_d0].
+  destruct (get_memory_cmp memory_cmp_tag) as [smemory_cmp H_smemory_cmp_snd].
+  destruct (get_storage_cmp storage_cmp_tag) as [sstorage_cmp H_sstorage_cmp_snd].
+  destruct (get_sha3_cmp sha3_cmp_tag) as [ssha3_cmp H_ssha3_cmp_snd].
+
+  unfold eq_block_chkr_snd.
+  intros p1 p2 ctx sst H_apply_chkr.
+  rewrite <- H_chkr in H_apply_chkr.
+  pose proof (evm_eq_block_chkr'_snd smemory_updater sstorage_updater mload_solver sload_solver sstack_value_cmp smemory_cmp sstorage_cmp ssha3_cmp (get_pipeline optimization_steps) opt_step_rep opt_pipeline_rep H_smemory_updater_snd H_sstorage_updater_snd H_mload_solver_snd H_sload_solver_snd H_sstack_value_cmp_snd_d0 H_smemory_cmp_snd H_sstorage_cmp_snd H_ssha3_cmp_snd H_sstack_value_cmp_snd) as H_evm_eq_block_chkr'_snd.
+  unfold eq_block_chkr_snd in H_evm_eq_block_chkr'_snd.
+  apply H_evm_eq_block_chkr'_snd.
+  apply H_apply_chkr.
+Qed.
+
+
+Lemma evm_eq_block_chkr_snd:
+  forall (memory_updater_tag: available_smemory_updaters) (storage_updater_tag: available_sstorage_updaters) (mload_solver_tag: available_mload_solvers) 
+  (sload_solver_tag: available_sload_solvers) (sstack_value_cmp_tag: available_sstack_val_cmp) (memory_cmp_tag: available_memory_cmp)
+  (storage_cmp_tag: available_storage_cmp) (sha3_cmp_tag: available_sha3_cmp) (optimization_steps: list_opt_steps) (opt_step_rep: nat) (opt_pipeline_rep: nat),
+    eq_block_chkr_snd (evm_eq_block_chkr memory_updater_tag storage_updater_tag mload_solver_tag sload_solver_tag sstack_value_cmp_tag memory_cmp_tag storage_cmp_tag sha3_cmp_tag optimization_steps opt_step_rep opt_pipeline_rep).
+Proof.
+  intros.  
+  unfold eq_block_chkr_snd.
+  unfold evm_eq_block_chkr.
+  remember (evm_eq_block_chkr_lazy memory_updater_tag storage_updater_tag mload_solver_tag sload_solver_tag sstack_value_cmp_tag memory_cmp_tag storage_cmp_tag sha3_cmp_tag optimization_steps opt_step_rep opt_pipeline_rep) as chkr.
+  symmetry in Heqchkr.
+
+  pose proof (evm_eq_block_chkr_lazy_snd memory_updater_tag storage_updater_tag mload_solver_tag sload_solver_tag sstack_value_cmp_tag memory_cmp_tag storage_cmp_tag sha3_cmp_tag optimization_steps opt_step_rep opt_pipeline_rep chkr Heqchkr) as H_evm_eq_block_chkr_lazy_snd.
+  apply H_evm_eq_block_chkr_lazy_snd.
+  
+Qed.
+
+
+End BlockEquivCheckerSoundness.
